\documentclass[letterpaper,12pt,titlepage,oneside,final]{book}
\usepackage{graphicx}
\usepackage{setspace}
\usepackage{fullpage}
\usepackage{amsmath,amsthm,amssymb}

%%Packages for graphs
\usepackage{pgf}
\usepackage{tikz}
\usetikzlibrary{arrows,automata}
\usepackage[latin1]{inputenc}

%Package for multi column
\usepackage{multicol}

%%Pure laziness.
\newcommand{\N}{\mathbb{N}}
\newcommand{\Z}{\mathbb{Z}}
\newcommand{\R}{\mathbb{R}}
\newcommand{\Q}{\mathbb{Q}}
\newcommand{\C}{\mathbb{C}}
\newcommand{\GN}{\mathcal{N}}

% TITLE PAGE GUBBINS
%----------------------------------------------------------------------
\newcommand{\thetitle}{Assignment 1}%Change title here
\newcommand{\coursecode}{MTH712}%Change course code here
\newcommand{\thedate}{\today}%Change the due date here


\begin{document}
% Title Page
%----------------------------------------------------------------------
\input{titlepage}
%----------------------------------------------------------------------


% Start Assignment
%----------------------------------------------------------------------


\section*{Question 1}

\begin{align*}
\text{Let $\mu(t)$ be such that }\quad
\mu(t) a &= \mu'(t)\\
a &= \frac{\mu'(t)}{\mu(t)}\\
&=\frac{d}{dt}\left(\ln(\mu (t)) \right)\\
\text{then,  }\quad 
\ln(\mu (t) &= \int a dt\\
& = at + C_1 \\
\text{and,  }\quad 
\mu(t) &=  C_1 e^{at} \quad \text{ (*)}\\
\\
\text{Now, }\quad
\mu(t)\frac{du}{dt} + \mu(t) au &= \mu(t) e^{at}\\
\mu(t)\frac{du}{dt} + \mu'(t)u &= \mu(t) e^{at}\\
\\
\text{By the product rule, }\quad
\frac{d}{dt}(\mu(t)u(t)) &= \mu(t) e^{at}\\
\\
\int\frac{d}{dt}(\mu(t)u(t))dt &= \int\mu(t) e^{at}dt\\
\mu(t)u(t)) + C_2 &= \int\mu(t) e^{at}dt\\
u(t)& = \frac{\int\mu(t) e^{at}dt + C_2}{\mu(t)}\\
& = \frac{\int\mu(t) e^{at}dt + C_2}{\mu(t)}\\
\text{then, } \quad 
u(t)& = \frac{C_1 \int  e^{at} e^{at}dt + C_3}{C_1 e^{at}} \quad \text{by (*) }\\
\\
\text{By substitution, }
\quad u(t)& = \frac{(e^{at})^2 + C_4}{2ae^{at}} \\
\\
\text{Hence, } 
\quad u(t) &= \frac{e^{at}}{K_1} + \frac{K_2}{e^{at}} \\
\end{align*}
\clearpage 


\section*{Question 2}
\begin{align*}
\frac{d^2u}{dx^2} - u\gamma^2 + \gamma^2 T &= 0\quad \text{where $\gamma, T$ are constants}\\
\frac{d^2u}{dx^2} - u\gamma^2 &= - \gamma^2 T \quad \text{(*)}\\
\\
\text{Using the auxillary equation, }\quad U = e^{mx}\\
\text{Now, }\quad m^2 - \gamma^2 = 0\\
(m + \gamma)(m - \gamma)=0\\
\text{Hence }\quad m = \pm \gamma\\
\\
\text{So, }\quad U_c &= C_1 e^{\gamma x} + C_2e^{-\gamma x}\\
\\
\text{Using undetermined coefficients: }\\
\text{Let $U_p = K \quad$, where K is a constant}\\
\\
\text{Now, sub into (*)}\\
\text{So, }\quad -\gamma^2 D &= -\gamma^2 T\\
D &= T\\
\text{and, }\quad U_p &= T\\
\\
\text{Hence, the general solutions is, }\quad \\
U(x) = U_c + U_p &= C_1 e^{\gamma x} + C_2e^{-\gamma x} + T
\end{align*}

\clearpage 


\section*{Question 3}
\begin{align*}
\frac{d}{dx}\left[(h + k x) \frac{dv}{dx} \right] &= 0\\
\\
\int \frac{d}{dx}\left[(h + k x) \frac{dv}{dx} \right] &= \int 0 dx \\
(h + k x) \frac{dv}{dx} & = C_1 \quad \text{where $C_1$ is some constant}\\
\\
\text{Now, }\quad  dv &= \frac{C_1}{h + k x}dx\\
\int dv &= \int \frac{C_1}{h + k x}dx\\
\\
\text{Hence, }\quad v &= C_1 \int \frac{dx}{h + k x}\\
& = C_1 \frac{\ln |h + kx|}{k} + C_2\\
\end{align*}

\clearpage


\section*{Question 4}
\begin{align*}
t^2 \frac{d^2u}{dt^2} + 2t \frac{du}{dt} -q(q+1)u &= 0\text{ (*)} \quad \text{Where, $t>0$ , q is a positive constant}\\
\\
&\text{Now,}\quad u = t^m\\
&\text{So, }\quad \frac{du}{dt} = mt^{m-1}\\
&\text{and, }\quad \frac{d^2u}{dt^2} = (m)(m-1)t^{m-2}\\
\\
\text{Now substituting into (*)}\\
t^2 \frac{d^2u}{dt^2} + 2t \frac{du}{dt} -q(q+1)u &= (m)(m-1)t^{m} + 2 mt^{m} -q(q+1)t^m \\
&= t^m \left[ m(m-1) + 2m -q(q+1)\right]\\
&= t^m \left[ m^2 + m - (q^2 +q)\right] = 0 \\
\\
&\text{So, $\quad t^m = 0$ and $ m^2 + m - (q^2 +q) = 0$}\\
\\
\text{Now, }\quad m^2 + m &= q^2 +q\\ 
m^2 + m + \frac{1}{4} & = q^2 +q + \frac{1}{4}\\  
\left(m+\frac{1}{2}\right)^2 &= \left( q + \frac{1}{2} \right)^2 \\
\left[m+\frac{1}{2} +  q + \frac{1}{2} \right]\left[m+\frac{1}{2} - q - \frac{1}{2} \right]& = 0\\
&\text{So, $ m = q$ and $m = -(q+1)$}\\
\\
\text{Hence, } u =  C_1 t^q + C_2 t^{-(q+1)}
\end{align*}
\clearpage

\section*{Question 5}
\begin{align*}
\frac{d^2u}{dx^2} -au = 0 \quad 0 < x < 1 \\
\frac{du}{dx} (0) = 0\\
u(1) = 1\\
\\
&\text{Using the auxillary equation, }\quad u = e^{mx}\\
&\text{Now, }\quad m^2 - a = 0\\
\text{Hence }\quad m = \pm \sqrt{a}\\
\text{So, }\quad U_c &= C_1 e^{\sqrt{a} x} + C_2e^{-\sqrt{a} x} \quad \text{(*)}\\
\\
&\text{Recall, }\\
&\cosh x = \frac{e^x + e^{-x}}{2}\quad \frac{d}{dx} \cosh x = \sinh x\\
&\sinh x = \frac{e^x - e^{-x}}{2} \quad \frac{d}{dx} \sinh x = \cosh x\\
\end{align*}
\begin{align*}
\text{Now, substitution into (*)}\\
U_c & = \left( C_1 + C_2 \right)\cosh (\sqrt{a}x) + \left( C_1 - C_2 \right)\sinh (\sqrt{a}x)\\
\text{Using the initial conditions, }\\
\frac{du}{dx}(0) &= \left( C_1 + C_2 \right) \sqrt{a}\sinh (\sqrt{a}0) + \left( C_1 - C_2 \right) \sqrt{a}\cosh (\sqrt{a}0)\\
&=\left( C_1 - C_2 \right)\sqrt{a} = 0\\
\text{So, } \quad C_1 = C_2\\
\\
\text{Also, }\quad u(1) &= \left( C_1 + C_2 \right)\cosh (\sqrt{a}(1)) + \left( C_1 - C_2 \right)\sinh (\sqrt{a}(1))\\
\\
\text{So, }\quad 1 = 2C_1\cosh(\sqrt{a})\\
\\
\text{From this, }\quad C_1 = C_2 = \frac{1}{2\cosh(\sqrt{a})}\\
\\
\text{Hence, }\quad
u(x) & = \frac{\cosh(\sqrt{a}x)}{\cosh(\sqrt{a})}
\end{align*}
\end{document}
