\documentclass[letterpaper,12pt,titlepage,oneside,final]{book}
\usepackage{graphicx}
\usepackage{setspace}
\usepackage{fullpage}
\usepackage{amsmath,amsthm,amssymb}

%%Packages for graphs
\usepackage{pgf}
\usepackage{tikz}
\usetikzlibrary{arrows,automata}
\usepackage[latin1]{inputenc}

%Package for multi column
\usepackage{multicol}

%%Pure laziness.
\newcommand{\N}{\mathbb{N}}
\newcommand{\Z}{\mathbb{Z}}
\newcommand{\R}{\mathbb{R}}
\newcommand{\Q}{\mathbb{Q}}
\newcommand{\C}{\mathbb{C}}
\newcommand{\cis}{\text{cis}}
\newcommand*{\pd}[3][]{\ensuremath{\frac{\partial^{#1} #2}{\partial #3}}}
\newcommand*{\ld}[3][]{\ensuremath{\frac{d^{#1} #2}{d #3}}}


% TITLE PAGE GUBBINS
%----------------------------------------------------------------------
\newcommand{\thetitle}{Assignment 1}%Change title here
\newcommand{\coursecode}{MTH712}%Change course code here
\newcommand{\thedate}{\today}%Change the due date here



\begin{document}
% Title Page
%----------------------------------------------------------------------
\input{titlepage}
%----------------------------------------------------------------------


% Start Assignment
%----------------------------------------------------------------------
\section*{1}
\begin{align*}
\text{Given, }&\quad \pd{u}{t}=\pd[2]{u}{x^2} - rx, \quad 0<x<L \quad t>0\\
\text{and BC: }&\quad \pd{u}{x}(0,t), \quad \pd{u}{x}(L,t) = \alpha, \\
&\text{Where, r and $\alpha$  are constants.}\\
\end{align*}

\paragraph{a)}
\begin{align*}
&\text{The corresponding time independent problem is:}\\
&0 = \pd[2]{u}{x^2} - rx, \quad 0<x<L\\
&\text{with BC:}\quad \pd{u}{x}(0) = 0, \quad \pd{u}{x}(L) = \alpha\\
\end{align*}
\begin{align*}
\text{Now, }\quad \int rx dx &= \int\pd[2]{u}{x^2} dx\\
\pd{u}{x} &= \frac{rx^2}{2} + K\\
\end{align*}
\begin{align*}
\text{So, }\quad \pd{u}{x}(0) &\implies \frac{r(0)^2}{2} +K = 0\quad\text{ie, }K=0\\
\text{And, }\quad \pd{u}{L} &\implies \frac{rL^2}{2}  = \alpha\\
&\text{Now, for a solution to exist, we must have}\quad r = \frac{2\alpha}{L^2} 
\end{align*}
\begin{align*}
\text{Hence, the general solution is, }\quad \pd{u}{x} &= \frac{\alpha x^2}{L^2}\\
\text{and, } U_E(X) = \int\pd{u}{x} dx =\int\frac{\alpha x^2}{L^2} dx= \frac{\alpha x^3}{3L^2} +K_2
\end{align*}


\paragraph{b)}
\begin{align*}
\text{From the previous relationship,}&\quad U(x,o) = f(x), \quad 0<x<L\\
\int_{0}^{L}\pd{u}{t}dx &= \int_{0}^{L}\pd[2]{u}{x^2}dx - \left.\frac{\alpha x^2}{L^2}\right|_{0}^{L} \quad \text{from }r = \frac{2\alpha}{L^2}\\
& = \left(\pd{u}{x}(L,t) - \pd{u}{x}(0,t)\right) - \left(\frac{\alpha L^2}{L^2} - \frac{\alpha (0)^2}{L^2} \right) \\
&= \alpha -0 -\alpha-0 =0
\end{align*}
\begin{align*}
\text{Now, }\quad \ld{}{t}\int_{0}^{L} U(x,t) dx &= 0,\quad t>0\\
\text{So, }\quad \int_{0}^{L} U(x,t)dx &= P \quad \text{, where $P$ is a constant}\\
\text{And, }\quad \int_{0}^{L} U(x,t)dx &= \int_{0}^{L} U_E(X) dx = \int_{0}^{L} \left(\frac{\alpha x^3}{3L^2} +K_2\right)dx\\
& = \left[\frac{\alpha x^4}{12 L^2} +K_2x \right]_{0}^{L}\\
\\
\text{Hence, }\quad \int_{0}^{1}f(x) dx &= \frac{\alpha L^4}{12L^2} + K_2L\\
\text{And the steady-state solution is } U_E(x) &= \frac{\alpha x^3}{3 L^2} + \frac{1}{L}\int_{0}^{L}f(x)dx -\frac{\alpha}{12}
\end{align*}
\cleardoublepage

\section*{2}
\begin{align*}
f(n) =
\begin{cases}
	x      & \quad \text{if }\quad -2<x<0\\
	1+x    & \quad \text{if }\quad 0<x<2
\end{cases}
\end{align*}
\cleardoublepage

\section*{4}
\begin{align*}
&g(y) \approx a_0 + \sum_{n=1}^{\infty}\left(a_n \cos\lambda_n(y) + b_n \sin \lambda_n (y)\right)\\
&\text{Let $f(x)$ denote $g(y)$ in terms of x and, } y = \frac{a+b}{2} + \frac{b-a}{2L}x\\
&\text{So, }f(x)\approx  a_0 + \sum_{n=1}^{\infty}\left(a_n \cos\left(\frac{n\pi}{L}x\right) + b_n \sin \left(\frac{n\pi}{L}x\right) \right)\\
\end{align*}
\begin{align*}
\text{Now, }\quad a_0 &= \frac{1}{2L}\int_{-L}^{-L}f(x)dx = \frac{1}{2L}\int_{-L}^{L}\left(\frac{a+b}{2} + \frac{b-a}{2L}x\right)dx\\
& = \frac{1}{2L} \left[\frac{a+b}{2}x + \frac{b-a}{4L}x^2\right]_{x=-L}^{x=L}\\
& = \frac{1}{2L}L(a+b) = \frac{a+b}{2}
\\
\text{and, }\quad a_n &= \frac{1}{L}\int_{-L}^{L}\left(\frac{a+b}{2}+\frac{b-a}{2L}x\right)\cos\left(\frac{n\pi}{L}x\right)dx\\
& = 
\end{align*}
\cleardoublepage

\end{document}
